---
layout: post
title: "Lessons from the Maths Teacher Blog-o-Sphere #1"
date: "2018-03-07 08:46:09"
categories: blog
tags: []
---
[From David Butler](https://twitter.com/DavidKButlerUoA/status/970569836009988097)

<blockquote class="twitter-tweet" data-width="550" data-dnt="true"><p lang="en" dir="ltr">Ohhhh. I’ve just realised another way to explain why negative*negative is positive. <br>For example:<br>(-3)*(-2)+(-3)*2<br>=(-3)*(-2+2)<br>=(-3)*0<br>=0<br>But (-3)*2=-6 (Students don’t seem to have a problem with neg*pos=neg.)<br>So (-3)*(-2)+(-6)=0.<br>Which means you must have<br>(-3)*(-2)=6.</p>&mdash; David Butler (@DavidKButlerUoA) <a href="https://twitter.com/DavidKButlerUoA/status/970569836009988097?ref_src=twsrc%5Etfw">March 5, 2018</a></blockquote><script async src="https://platform.twitter.com/widgets.js" charset="utf-8"></script>